@prefix : <https://w3id.org/i40/rami#> .
@prefix dc: <http://purl.org/dc/elements/1.1/> .
@prefix om: <http://www.wurvoc.org/vocabularies/om-1.8/> .
@prefix DUL: <http://www.loa-cnr.it/ontologies/DUL.owl#> .
@prefix dul: <http://www.loa-cnr.it/ontologies/DUL.owl#> .
@prefix geo: <http://www.w3.org/2003/01/geo/wgs84_pos#> .
@prefix owl: <http://www.w3.org/2002/07/owl#> .
@prefix rdf: <http://www.w3.org/1999/02/22-rdf-syntax-ns#> .
@prefix ssn: <http://purl.oclc.org/NET/ssnx/ssn#> .
@prefix sto: <https://w3id.org/i40/sto#> .
@prefix xml: <http://www.w3.org/XML/1998/namespace> .
@prefix xsd: <http://www.w3.org/2001/XMLSchema#> .
@prefix foaf: <http://xmlns.com/foaf/spec/> .
@prefix obda: <https://w3id.org/obda/vocabulary#> .
@prefix prov: <http://www.w3.org/ns/prov#> .
@prefix rami: <https://w3id.org/i40/rami#> .
@prefix rdfs: <http://www.w3.org/2000/01/rdf-schema#> .
@prefix skos: <http://www.w3.org/2004/02/skos/core#> .
@prefix vann: <http://purl.org/vocab/vann/> .
@prefix void: <http://rdfs.org/ns/void#> .
@prefix vcard: <http://www.w3.org/2006/vcard/ns#> .
@prefix dcterms: <http://purl.org/dc/terms/> .
@base <https://w3id.org/i40/rami/> .


###  http://purl.oclc.org/NET/ssnx/ssn#Sensor
ssn:Sensor rdf:type owl:Class .


###  http://purl.oclc.org/NET/ssnx/ssn#SensorOutput
ssn:SensorOutput rdf:type owl:Class ;
                 owl:equivalentClass rami:SensorMeasurementData .


###  http://www.w3.org/ns/prov#Agent
prov:Agent rdf:type owl:Class .


###  http://www.wurvoc.org/vocabularies/om-1.8/Measure
om:Measure rdf:type owl:Class .


###  http://www.wurvoc.org/vocabularies/om-1.8/Unit
om:Unit rdf:type owl:Class .


###  http://xmlns.com/foaf/spec/Image
foaf:Image rdf:type owl:Class .

###  https://w3id.org/i40/rami#CumulativeEnergyConsumption
rami:CumulativeEnergyConsumption rdf:type owl:Class .


###  https://w3id.org/i40/rami#EnergyEfficiency
rami:EnergyEfficiency rdf:type owl:Class ;
                      rdfs:subClassOf rami:Submodel .

###  https://w3id.org/i40/rami#MESConnection
rami:MESConnection rdf:type owl:Class ;
                   rdfs:subClassOf rami:Submodel .

###  https://w3id.org/i40/rami#energyEfficiencyValue
rami:energyEfficiencyValue rdf:type owl:ObjectProperty ;
                           rdfs:domain rami:EnergyEfficiency ;
                           rdfs:range om:Measure ;
                           rdfs:comment "Points to the value of the Energy Efficiency comsuption."@en ;
                           rdfs:label "energy Efficiency Value"@en .

###  https://w3id.org/i40/rami#hasAccessControlPolicyPoints
rami:hasAccessControlPolicyPoints rdf:type owl:ObjectProperty ;
                                  rdfs:comment "Access control policy points of the AAS."@en ;
                                  rdfs:label "has accessControlPolicyPoints"^^xsd:string .


###  https://w3id.org/i40/rami#hasComponentManager
rami:hasComponentManager rdf:type owl:ObjectProperty ;
                         rdfs:domain rami:AdminShell ;
                         rdfs:range rami:ComponentManager ;
                         rdfs:label "has Component Manager"@en .



###  https://w3id.org/i40/rami#SensorMeasurement
rami:SensorMeasurement rdf:type owl:Class ;
                       rdfs:subClassOf rami:Submodel .


###  https://w3id.org/i40/rami#SensorMeasurementData
rami:SensorMeasurementData rdf:type owl:Class ;
                           rdfs:comment "Data measured by a sensor"@en ;
                           rdfs:label "Sensor Data"@en .

###  http://www.wurvoc.org/vocabularies/om-1.8/hertz
om:hertz rdf:type owl:NamedIndividual .


###  http://www.wurvoc.org/vocabularies/om-1.8/kilojoule
om:kilojoule rdf:type owl:NamedIndividual .


###  http://www.wurvoc.org/vocabularies/om-1.8/kilowattHour
om:kilowattHour rdf:type owl:NamedIndividual .


###  http://www.wurvoc.org/vocabularies/om-1.8/ohm
om:ohm rdf:type owl:NamedIndividual .


###  https://w3id.org/i40/rami#AdminShell1
rami:AdminShell1 rdf:type owl:NamedIndividual ,
                          rami:AdminShell ;
                 rami:hasSubmodel rami:EnergyEfficiency1 ;
                 rami:hasAdminShellId "AAS111"^^xsd:string ;
                 rdfs:label "Admin Shell 1"@en .


###  https://w3id.org/i40/rami#AdminShell2
rami:AdminShell2 rdf:type owl:NamedIndividual ,
                          rami:AdminShell ;
                 rami:hasSubmodel rami:EnergyEfficiency2 ;
                 rami:hasAdminShellId "AAS112"^^xsd:string ;
                 rdfs:label "Admin Shell 2"@en .


###  https://w3id.org/i40/rami#AdminShellMotor
rami:AdminShellMotor rdf:type owl:NamedIndividual ,
                              rami:AdminShell ;
                     rami:describes rami:AssetMotorControl ;
                     rdfs:label "Admin Shell Motor"@en .


###  https://w3id.org/i40/rami#Asset1
rami:Asset1 rdf:type owl:NamedIndividual ,
                     rami:Asset ;
            rami:hasAssetId "AS711"^^xsd:string ;
            rdfs:label "Asset 1"@en .


###  https://w3id.org/i40/rami#Asset2
rami:Asset2 rdf:type owl:NamedIndividual ,
                     rami:Asset ;
            rami:hasAssetId "AS712"^^xsd:string ;
            rdfs:label "Asset 2"@en .


###  https://w3id.org/i40/rami#AssetInstanceProductionPhase
rami:AssetInstanceProductionPhase rdf:type owl:NamedIndividual ,
                                           rami:LifeCycleDimension ;
                                  rdfs:comment "The production phase of asset instances. Asset instances are created/ produced, based on the asset type information. Specific information about production, logistics, qualification and test are associated with the asset instances."@en ;
                                  rdfs:label "Production"@en ;
                                  skos:altLabel "Asset Instance Production Phase"@en .


###  https://w3id.org/i40/rami#AssetInstanceUsageMaintenancePhase
rami:AssetInstanceUsageMaintenancePhase rdf:type owl:NamedIndividual ,
                                                 rami:LifeCycleDimension ;
                                        rdfs:comment """The asset instance usage and maintenance phase. Usage phase by the purchaser of the asset instances. Usage data is associated with the asset instance and might be shared with other value chain partners, such as the manufacturer of the asset instance. Also included: maintenance, re-design, optimization and decommissioning of the asset instance. The full life-cycle history is
associated with the asset and might be archived/ shared for
documentation."""@en ;
                                        rdfs:label "Usage/Maintenance"@en ;
                                        skos:altLabel "Asset Instance Usage/Maintenance Phase"@en .


###  https://w3id.org/i40/rami#AssetMotorControl
rami:AssetMotorControl rdf:type owl:NamedIndividual ,
                                rami:Asset ;
                       rami:hasAssetId "1501325"^^xsd:string ;
                       rdfs:label "Motor control"@en .


###  https://w3id.org/i40/rami#AssetTypeDevelopmentPhase
rami:AssetTypeDevelopmentPhase rdf:type owl:NamedIndividual ,
                                        rami:LifeCycleDimension ;
                               rdfs:comment """The development phase of asset types. Valid from the ideation/ conceptualization to first prototypes/ test. The 'type' of an asset is defined, and distinguishing properties and functionalities are defined and implemented. All (internal) design artefacts are created, such as CAD data, schematics, embedded
software, and associated with the asset type."""@en ;
                               rdfs:label "Development"@en ;
                               skos:altLabel "Asset Type Development Phase"@en .


###  https://w3id.org/i40/rami#AssetTypeUsageMaintenancePhase
rami:AssetTypeUsageMaintenancePhase rdf:type owl:NamedIndividual ,
                                             rami:LifeCycleDimension ;
                                    rdfs:comment "The usage and maintenance phase of asset types. Ramping up production capacity. The 'external' information associated to the asset is created, such as technical data sheets, marketing information. The selling process starts."@en ;
                                    rdfs:label "Usage/Maintenance"@en ;
                                    skos:altLabel "Asset Type Usage/Maintenance Phase"@en .


###  https://w3id.org/i40/rami#BrakingResistanceMs
rami:BrakingResistanceMs rdf:type owl:NamedIndividual ,
                                  om:Measure ;
                         om:hasUnit om:ohm ;
                         om:hasNumericalValue "60.0"^^xsd:float .


###  https://w3id.org/i40/rami#EnergyEfficiency1
rami:EnergyEfficiency1 rdf:type owl:NamedIndividual ,
                                rami:EnergyEfficiency ;
                       rami:energyEfficiencyValue rami:MeasureEnergyEfficiency1 ;
                       rami:hasView rami:Performance ;
                       rami:subModelID "AAB012"^^xsd:string ;
                       rdfs:label "Energy Efficiency 1 Submodel"@en ;
                       skos:definition "Integrated electrical consumption over time."@en ;
                       skos:prefLabel "Electrical consumption cumulative energy"@en ;
                       rami:semanticId rami:Measurement .


###  https://w3id.org/i40/rami#EnergyEfficiency2
rami:EnergyEfficiency2 rdf:type owl:NamedIndividual ,
                                rami:EnergyEfficiency ;
                       rami:energyEfficiencyValue rami:MeasureEnergyEfficiency2 ;
                       rami:subModelID "AAB013"^^xsd:string ;
                       rdfs:label "Energy Efficiency 2 Submodel"@en .


###  https://w3id.org/i40/rami#Platform1
rami:Platform1 rdf:type owl:NamedIndividual .

###  https://w3id.org/i40/rami#maxOutputFrequencyMs
rami:maxOutputFrequencyMs rdf:type owl:NamedIndividual ,
                                   om:Measure ;
                          om:hasUnit om:hertz ;
                          om:hasNumericalValue "1.0"^^xsd:float .





###  https://w3id.org/i40/rami#MeasureEnergyEfficiency1
rami:MeasureEnergyEfficiency1 rdf:type owl:NamedIndividual ,
                                       om:Measure ;
                              owl:sameAs rami:MeasureEnergyEfficiency2 ;
                              om:hasUnit om:kilowattHour ;
                              rdfs:comment "Measuring the Energy Efficiency for I4.0 component 1 in kilowattHour."@en ;
                              rdfs:label "Measure Energy Efficiency 1"@en ;
                              om:hasNumericalValue "17.3"^^xsd:float .


###  https://w3id.org/i40/rami#MeasureEnergyEfficiency2
rami:MeasureEnergyEfficiency2 rdf:type owl:NamedIndividual ,
                                       om:Measure ;
                              om:hasUnit om:kilojoule ;
                              rdfs:comment "Measuring the Energy Efficiency for I4.0 component 2 in Kilojoule."@en ;
                              rdfs:label "Measure Energy Efficiency 2"@en ;
                              om:hasNumericalValue "62280.0"^^xsd:float .
							  
							  
###  https://w3id.org/i40/rami#TechnicalData1
rami:TechnicalData1 rdf:type owl:NamedIndividual ;
                    rdfs:label "Technical Data 1"@en ;
                    rami:display "Seven-segment display"@en .

###  https://w3id.org/i40/rami#I4.0Component1
rami:I4.0Component1 rdf:type owl:NamedIndividual ,
                             rami:I4.0Component ;
                    rami:containsAS rami:AdminShell2 ;
                    rami:hasI40ComponentId "I40C112"^^xsd:string ;
                    rdfs:label "I4.0 Component 2"@en .


###  https://w3id.org/i40/rami#I4.0Component2
rami:I4.0Component2 rdf:type owl:NamedIndividual ,
                             rami:I4.0Component ;
                    rami:containsAS rami:AdminShell1 ;
                    rami:hasI40ComponentId "I40C111"^^xsd:string ;
                    rdfs:label "I4.0 Component 1"@en .



###  https://w3id.org/i40/rami#inventoryNumber
rami:inventoryNumber rdf:type owl:DatatypeProperty ,
                              owl:FunctionalProperty ;
                     rdfs:domain rami:Asset ;
                     rdfs:range xsd:string ;
                     skos:definition "Inventory number of the Entity/Object according to the identification nomenclature"@en ;
                     skos:prefLabel "Inventory Number"@en .


###  https://w3id.org/i40/rami#Machine
rami:Machine rdf:type owl:Class ;
             rdfs:subClassOf rami:Asset ;
             skos:definition "A machine is ordered, designed, commissioned, operated, serviced, converted and recycled."@en ;
             skos:prefLabel "Machine"@en .